Uppaal_Networks/UPPAAL_Asm_AbsInt_MapRefine.thy
@@ -1,7 +1,7 @@
 theory UPPAAL_Asm_AbsInt_MapRefine
 imports                   
   "HOL-Library.RBT_Mapping"
-  UPPAAL_Asm_AbsInt
+  UPPAAL_Asm_AbsInt_State_Dumb
 begin
 
 type_synonym 'a r_state_map = "(addr, 'a) mapping"
@@ -16,8 +16,10 @@ declare RSM_def[simp]
 
 code_datatype RSM
 
-lemma[code]: "empty_map = RSM (Mapping.empty::('a::bot) r_state_map)"
-  by (rule lookup_eq; simp add: empty_map_def lookup_default_empty)
+definition "r_empty_map \<equiv> Mapping.empty::('a::bot) r_state_map"
+
+lemma[code]: "empty_map = RSM r_empty_map"
+  by (rule lookup_eq; simp add: empty_map_def lookup_default_empty r_empty_map_def)
 
 lemma[code]: "lookup (RSM m) = r_lookup m" by simp
 
@@ -31,7 +33,7 @@ lemma merge_single_neq:
   assumes "pc \<noteq> k"
   shows "lookup (RSM (r_merge_single m pc x)) k = lookup (RSM m) k"
 proof -
-  have r: "lookup (RSM m) k = Mapping.lookup_default \<bottom> m k" by (simp add: RSM_def)
+  have r: "lookup (RSM m) k = Mapping.lookup_default \<bottom> m k" by simp
   from assms have l:"lookup (RSM (r_merge_single m pc x)) k = Mapping.lookup_default \<bottom> m k" by (simp add: lookup_default_update_neq) 
   from r l show ?thesis by simp
 qed
@@ -68,6 +70,47 @@ proof (intro Set.equalityI Set.subsetI)
     by (metis Option.is_none_def empty_iff keys_empty keys_is_none_rep lookup_default_def lookup_default_empty r_lookup.simps)
   from keys r_lookup show "x \<in> r_domain m" by auto
 qed auto
+
+fun r_step_map_from :: "('a::absstate) astep \<Rightarrow> instr \<Rightarrow> addr \<Rightarrow> 'a state_map \<Rightarrow> 'a state_map" where
+  "r_step_map_from f op ipc ctx = fold
+    (\<lambda>pc acc. merge_single acc pc (f op ipc (lookup ctx ipc) pc))
+    (sorted_list_of_set (astep_succs f op ipc (lookup ctx ipc))) ctx"
+
+fun r_step_map :: "('a::absstate) astep \<Rightarrow> program \<Rightarrow> 'a state_map \<Rightarrow> 'a state_map" where
+  "r_step_map f prog ctx = fold
+    (\<lambda>ipc acc. case prog ipc of
+      Some op \<Rightarrow> r_step_map_from f op ipc acc |
+      None \<Rightarrow> acc)
+    (sorted_list_of_set (domain ctx)) empty_map"
+
+fun r_advance :: "('a::{semilattice_sup, Sup}) astep \<Rightarrow> program \<Rightarrow> 'a r_state_map \<Rightarrow> 'a r_state_map" where
+  "r_advance f prog ctx = undefined"
+
+
+fun dumb_step :: "dumb astep" where
+  "dumb_step _ _ None _ = None" |
+  "dumb_step (JMPZ target) ipc ins pc = (if pc = Suc ipc \<or> pc = target then Some Any else None)" |
+  "dumb_step CALL ipc ins pc = Some Any" |
+  "dumb_step RETURN ipc ins pc = Some Any" |
+  "dumb_step HALT ipc ins pc = None" |
+  "dumb_step _ ipc ins pc = (if pc = Suc ipc then Some Any else None)"
+
+(***********)
+lemma[code_unfold]: "astep_succs dumb_step op pc st =
+  (case (op, st) of
+    (_, None)        \<Rightarrow> {} |
+    (JMPZ target, _) \<Rightarrow> {target, pc + 1} |
+    (CALL, _)        \<Rightarrow> UNIV |
+    (RETURN, _)      \<Rightarrow> UNIV |
+    (HALT, _)        \<Rightarrow> {} |
+    _                \<Rightarrow> {pc + 1})"
+proof (cases st)
+  case None
+  then show ?thesis sorry
+next
+  case (Some a)
+  then show ?thesis sorry
+qed
 
 value "
   let m = empty_map::bool state_map;
